\documentclass{article}

\usepackage{amsmath}

\begin{document}

Problem 1

\[
f^{-1}(x) = \frac{x - 16}{40}
\]

Problem 2

\[
f^{-1}(x) = \frac{x - 43}{31}
\]

Problem 3

\[
f^{-1}(x) = \frac{x - 40}{14}
\]

Problem 4

\[
f^{-1}(x) = \frac{x - 16}{19}
\]

Problem 5

\[
f^{-1}(x) = \frac{x - 3}{48}
\]

Problem 6

\[
f^{-1}(x) = \frac{x - 45}{33}
\]

Problem 7

\[
f^{-1}(x) = \frac{x - 19}{1}
\]

Problem 8

\[
f^{-1}(x) = \frac{x - 21}{40}
\]

Problem 9

\[
f^{-1}(x) = \frac{x - 25}{44}
\]

Problem 10

\[
f^{-1}(x) = \frac{x - 41}{32}
\]

Problem 11

\[
f^{-1}(x) = \frac{x - 7}{30}
\]

Problem 12

\[
f^{-1}(x) = \frac{x - 1}{38}
\]

Problem 13

\[
f^{-1}(x) = \frac{x - 14}{47}
\]

Problem 14

\[
f^{-1}(x) = \frac{x - 34}{4}
\]

Problem 15

\[
f^{-1}(x) = \frac{x - 24}{12}
\]

Problem 16

\[
f^{-1}(x) = \frac{x - 34}{18}
\]

Problem 17

\[
f^{-1}(x) = \frac{x - 20}{30}
\]

Problem 18

\[
f^{-1}(x) = \frac{x - 8}{23}
\]

Problem 19

\[
f^{-1}(x) = \frac{x - 6}{43}
\]

Problem 20

\[
f^{-1}(x) = \frac{x - 28}{29}
\]

Problem 21

\[
f^{-1}(x) = \frac{x - 50}{48}
\]

Problem 22

\[
f^{-1}(x) = \frac{x - 16}{17}
\]

Problem 23

\[
f^{-1}(x) = \frac{x - 41}{45}
\]

Problem 24

\[
f^{-1}(x) = \frac{x - 22}{5}
\]

Problem 25

\[
f^{-1}(x) = \frac{x - 47}{38}
\]

Problem 26

\[
f^{-1}(x) = \frac{x - 18}{47}
\]

Problem 27

\[
f^{-1}(x) = \frac{x - 41}{49}
\]

Problem 28

\[
f^{-1}(x) = \frac{x - 34}{27}
\]

Problem 29

\[
f^{-1}(x) = \frac{x - 19}{2}
\]

Problem 30

\[
f^{-1}(x) = \frac{x - 24}{22}
\]

Problem 31

\[
f^{-1}(x) = \frac{x - 17}{48}
\]

Problem 32

\[
f^{-1}(x) = \frac{x - 43}{37}
\]

Problem 33

\[
f^{-1}(x) = \frac{x - 19}{32}
\]

Problem 34

\[
f^{-1}(x) = \frac{x - 46}{12}
\]

Problem 35

\[
f^{-1}(x) = \frac{x - 3}{9}
\]

Problem 36

\[
f^{-1}(x) = \frac{x - 23}{46}
\]

Problem 37

\[
f^{-1}(x) = \frac{x - 9}{35}
\]

Problem 38

\[
f^{-1}(x) = \frac{x - 37}{4}
\]

Problem 39

\[
f^{-1}(x) = \frac{x - 18}{16}
\]

Problem 40

\[
f^{-1}(x) = \frac{x - 33}{8}
\]

Problem 41

\[
f^{-1}(x) = \frac{x - 38}{17}
\]

Problem 42

\[
f^{-1}(x) = \frac{x - 11}{10}
\]

Problem 43

\[
f^{-1}(x) = \frac{x - 49}{29}
\]

Problem 44

\[
f^{-1}(x) = \frac{x - 50}{28}
\]

Problem 45

\[
f^{-1}(x) = \frac{x - 1}{7}
\]

Problem 46

\[
f^{-1}(x) = \frac{x - 38}{3}
\]

Problem 47

\[
f^{-1}(x) = \frac{x - 1}{5}
\]

Problem 48

\[
f^{-1}(x) = \frac{x - 35}{11}
\]

Problem 49

\[
f^{-1}(x) = \frac{x - 25}{50}
\]

Problem 50

\[
f^{-1}(x) = \frac{x - 14}{36}
\]

Problem 51

\[
f^{-1}(x) = \frac{x - 21}{34}
\]

Problem 52

\[
f^{-1}(x) = \frac{x - 45}{35}
\]

Problem 53

\[
f^{-1}(x) = \frac{x - 14}{40}
\]

Problem 54

\[
f^{-1}(x) = \frac{x - 44}{29}
\]

Problem 55

\[
f^{-1}(x) = \frac{x - 16}{17}
\]

Problem 56

\[
f^{-1}(x) = \frac{x - 26}{20}
\]

Problem 57

\[
f^{-1}(x) = \frac{x - 21}{28}
\]

Problem 58

\[
f^{-1}(x) = \frac{x - 7}{30}
\]

Problem 59

\[
f^{-1}(x) = \frac{x - 43}{2}
\]

Problem 60

\[
f^{-1}(x) = \frac{x - 44}{4}
\]

Problem 61

\[
f^{-1}(x) = \frac{x - 23}{5}
\]

Problem 62

\[
f^{-1}(x) = \frac{x - 32}{43}
\]

Problem 63

\[
f^{-1}(x) = \frac{x - 23}{3}
\]

Problem 64

\[
f^{-1}(x) = \frac{x - 33}{25}
\]

Problem 65

\[
f^{-1}(x) = \frac{x - 46}{49}
\]

Problem 66

\[
f^{-1}(x) = \frac{x - 47}{42}
\]

Problem 67

\[
f^{-1}(x) = \frac{x - 9}{10}
\]

Problem 68

\[
f^{-1}(x) = \frac{x - 9}{16}
\]

Problem 69

\[
f^{-1}(x) = \frac{x - 16}{39}
\]

Problem 70

\[
f^{-1}(x) = \frac{x - 39}{17}
\]

Problem 71

\[
f^{-1}(x) = \frac{x - 15}{43}
\]

Problem 72

\[
f^{-1}(x) = \frac{x - 13}{22}
\]

Problem 73

\[
f^{-1}(x) = \frac{x - 12}{45}
\]

Problem 74

\[
f^{-1}(x) = \frac{x - 43}{11}
\]

Problem 75

\[
f^{-1}(x) = \frac{x - 27}{34}
\]

Problem 76

\[
f^{-1}(x) = \frac{x - 32}{11}
\]

Problem 77

\[
f^{-1}(x) = \frac{x - 1}{1}
\]

Problem 78

\[
f^{-1}(x) = \frac{x - 13}{39}
\]

Problem 79

\[
f^{-1}(x) = \frac{x - 41}{16}
\]

Problem 80

\[
f^{-1}(x) = \frac{x - 45}{34}
\]

Problem 81

\[
f^{-1}(x) = \frac{x - 8}{14}
\]

Problem 82

\[
f^{-1}(x) = \frac{x - 38}{19}
\]

Problem 83

\[
f^{-1}(x) = \frac{x - 18}{5}
\]

Problem 84

\[
f^{-1}(x) = \frac{x - 4}{1}
\]

Problem 85

\[
f^{-1}(x) = \frac{x - 24}{19}
\]

Problem 86

\[
f^{-1}(x) = \frac{x - 38}{41}
\]

Problem 87

\[
f^{-1}(x) = \frac{x - 43}{39}
\]

Problem 88

\[
f^{-1}(x) = \frac{x - 26}{36}
\]

Problem 89

\[
f^{-1}(x) = \frac{x - 29}{48}
\]

Problem 90

\[
f^{-1}(x) = \frac{x - 17}{24}
\]

Problem 91

\[
f^{-1}(x) = \frac{x - 2}{17}
\]

Problem 92

\[
f^{-1}(x) = \frac{x - 4}{33}
\]

Problem 93

\[
f^{-1}(x) = \frac{x - 27}{49}
\]

Problem 94

\[
f^{-1}(x) = \frac{x - 22}{17}
\]

Problem 95

\[
f^{-1}(x) = \frac{x - 1}{42}
\]

Problem 96

\[
f^{-1}(x) = \frac{x - 22}{18}
\]

Problem 97

\[
f^{-1}(x) = \frac{x - 18}{28}
\]

Problem 98

\[
f^{-1}(x) = \frac{x - 20}{20}
\]

Problem 99

\[
f^{-1}(x) = \frac{x - 44}{1}
\]

Problem 100

\[
f^{-1}(x) = \frac{x - 9}{21}
\]

\end{document}